src/Std/Data/TreeMap/Basic.lean
@@ -21,7 +21,7 @@ nested inductive types.
 set_option autoImplicit false
 set_option linter.missingDocs true
 
-universe u v
+universe u v w w₂
 
 variable {α : Type u} {β : Type v} {cmp : α → α → Ordering}
 
@@ -142,7 +142,6 @@ instance : GetElem? (TreeMap α β cmp) α β (fun m a => a ∈ m) where
   getElem? m a := m.get? a
   getElem! m a := m.get! a
 
-universe w w₂
 variable {δ : Type w} {m : Type w → Type w₂} [Monad m]
 
 @[inline, inherit_doc DTreeMap.filter]
